template-coq/theories/TypingWf.v
@@ -347,7 +347,7 @@ Proof.
   eapply nth_error_alli in Hidecl; eauto. simpl in *.
   pose proof (onConstructors Hidecl) as h. unfold on_constructors in h.
   eapply All2_nth_error_Some in Hcdecl. 2: eassumption.
-  destruct Hcdecl as [? [? [[s [? ?]] [? ?]]]].
+  destruct Hcdecl as [? [? [[s ?] [? [? ?]]]]].
   assumption.
 Qed.
 
@@ -546,7 +546,7 @@ Proof.
   - destruct c; simpl. destruct cst_body; simpl in *.
     red in o |- *. simpl in *. now eapply X.
     red in o |- *. simpl in *. now eapply X.
-  - red in o. simpl in *.
+  - simpl in *.
     destruct o0 as [onI onP onNP].
     constructor; auto.
     -- eapply Alli_impl. exact onI. eauto. intros.
@@ -556,15 +556,19 @@ Proof.
        --- apply onArity in X1. unfold on_type in *; simpl in *.
            now eapply X.
        --- pose proof X1.(onConstructors) as X11. red in X11.
-           unfold on_constructor, on_type in *. eapply All2_impl; eauto.
-           simpl. intros. destruct X2 as (? & ? & ?).
-           split. now eapply X.
-           exists x1.
-           clear -t X X0.
-           revert t. generalize (cshape_args x1).
-           induction c; simpl; auto;
-           destruct a as [na [b|] ty]; simpl in *; auto;
+           eapply All2_impl; eauto.
+           simpl. intros. destruct X2 as [? ? ? ?]; unshelve econstructor; eauto.
+           * apply X; eauto.
+           * clear -X0 X on_cargs. revert on_cargs.
+              generalize (cshape_args cshape).
+              induction c; simpl; auto;
+              destruct a as [na [b|] ty]; simpl in *; auto;
            split; intuition eauto.
+           * clear -X0 X on_cindices.
+             revert on_cindices.
+             generalize (List.rev  (lift_context #|cshape_args cshape| 0 (ind_indices X1))).
+             generalize (cshape_indices cshape).
+             induction 1; simpl; constructor; auto.
        --- simpl; intros. pose (onProjections X1 H0). simpl in *.
            destruct o0. constructor; auto. eapply Alli_impl; intuition eauto.
            unfold on_projection in *; simpl in *.
